Finding denotational sweet spot

investigations/cava2/Fib.v
@@ -26,17 +26,20 @@ Require Import Cava.Semantics.
 
 Section Var.
   Import ExprNotations.
+  Import PrimitiveNotations.
   Context {var : tvar}.
 
   Definition fork2 {A} : Circuit [] [A] (A ** A) := {{
     fun a => (a, a)
   }}.
 
-  Definition fibonacci {sz: nat}: Circuit (Nat ** Nat) [] Nat := {{
+  Definition fib_init sz := const (BitVec sz) (2^(N.of_nat sz)-1)%N.
+
+  Definition fibonacci {sz: nat}: Circuit (BitVec sz ** BitVec sz) [] (BitVec sz) := {{
     let/delay r1 :=
-      let r2 := delay r1 initially (2^sz-1:denote_type Nat) in
-      `AddMod sz` r1 r2
-      initially (1:denote_type Nat) in
+      let r2 := delay r1 initially (fib_init sz) in
+      r1 + r2
+      initially (const (BitVec sz) 1%N) in
     r1
   }}.
 End Var.
@@ -58,53 +61,71 @@ Fixpoint fibonacci_nat (n : nat) :=
     end
   end.
 
-Definition spec_of_fibonacci (sz : nat) (input : list unit) : list nat
-  := map (fun n => fibonacci_nat n mod (2 ^ sz)) (seq 0 (List.length input)).
+Definition spec_of_fibonacci (sz : nat) (input : list unit) : list N
+  := map (fun n => N.of_nat (fibonacci_nat n) mod (2 ^ N.of_nat sz))%N (seq 0 (List.length input)).
 
 Lemma fork2_step A state input : step (fork2 (A:=A)) state (input, tt) = (tt, (input, input)).
 Proof. reflexivity. Qed.
-
+Open Scope N.
 Lemma fibonacci_step sz state input :
-  step (fibonacci (sz:=sz)) state input
-  = let sum := (fst state + snd state) mod (2 ^ sz) in
-    (sum, fst state, sum).
+  let (z1,z2) := step (fibonacci (sz:=sz)) state input in
+  (denote_to_denote1 z1, denote_to_denote1 z2)
+  = let state' := denote_to_denote1 state in
+    let sum := (fst state' + snd state') mod (2 ^ N.of_nat sz) in
+    (sum, fst state', sum).
 Proof.
-  intros; cbn [step fibonacci ].
-  repeat (destruct_pair_let; cbn [split_absorbed_denotation combine_absorbed_denotation List.app absorb_any fst snd]).
-  reflexivity.
-Qed.
+  intros; cbn [step fibonacci
+  denote1_to_denote denote_to_denote1
+  Bv2N Vector.of_list Primitives.binary_semantics
+  ].
+  repeat (destruct_pair_let; cbn [split_absorbed_denotation combine_absorbed_denotation List.app absorb_any fst snd
+  Bv2N Vector.of_list N.of_nat fst snd
+  ]).
+  assert (forall n x, (Bv2N (Vector.of_list (Vector.to_list (N2Bv_sized n x)))) = x).
+  {admit. }
 
-Definition fibonacci_invariant {sz}
-           (t : nat) (loop_state : nat * nat)
-           (output_accumulator : list nat) : Prop :=
+  rewrite H.
+  reflexivity.
+Admitted.
+
+
+Axiom Nto_list_bool: N -> list bool.
+Axiom Nof_list_bool: list bool -> N.
+
+Import ListNotations.
+Definition fibonacci_invariant {sz: nat}
+           (t : nat) (loop_state : list bool * list bool)
+           (output_accumulator : list (list bool)) : Prop :=
   let r1 := fst loop_state in
   let r2 := snd loop_state in
   (* at timestep t... *)
   (* ...r1 holds fibonacci_nat (t-1), or 1 if t=0 *)
   r1 = match t with
-       | 0 => 1
-       | S t_minus1 => (fibonacci_nat t_minus1) mod (2 ^ sz)
+       | 0%nat => [true]%list
+       | S t_minus1 => Nto_list_bool
+         (N.of_nat (fibonacci_nat t_minus1) mod (2 ^ N.of_nat sz))
        end
   (* ... and r2 holds fibonacci_nat (t-2), or 1 if t=1, 2^sz-1 if t=0 *)
   /\ r2 = match t with
-         | 0 => 2 ^ sz - 1
-         | 1 => 1
-         | S (S t_minus2) =>(fibonacci_nat t_minus2) mod (2 ^ sz)
+         | 0%nat => Nto_list_bool (2 ^ N.of_nat sz - 1)
+         | 1%nat => [true]
+         | S (S t_minus2) => N.of_nat(fibonacci_nat t_minus2) mod (2 ^ N.of_nat sz)
          end
   (* ... and the output accumulator matches the circuit spec for the
      inputs so far *)
   /\ output_accumulator = spec_of_fibonacci sz (repeat tt t).
 
-(* Helper lemma for fibonacci_correct *)
-Lemma fibonacci_nat_step n :
-  fibonacci_nat (S (S n)) = fibonacci_nat (S n) + fibonacci_nat n.
-Proof. cbn [fibonacci_nat]. lia. Qed.
+(* (1* Helper lemma for fibonacci_correct *1) *)
+(* Lemma fibonacci_nat_step n : *)
+(*   fibonacci_nat (S (S n)) = fibonacci_nat (S n) + fibonacci_nat n. *)
+(* Proof. cbn [fibonacci_nat]. lia. Qed. *)
 
 Lemma fibonacci_correct sz input :
-  simulate (fibonacci (sz:=sz)) input = spec_of_fibonacci sz input.
+  map (Nto_list_bool) (simulate (fibonacci (sz:=sz)) input) = spec_of_fibonacci sz input.
 Proof.
   cbv [simulate]. rewrite fold_left_accumulate_to_seq with (default:=tt).
-  assert (2 ^ sz <> 0) by (apply Nat.pow_nonzero; lia).
+  assert (2 ^ sz <> 0)%nat by (apply Nat.pow_nonzero; lia).
+  eapply fold_left_accumulate_invariant_seq with (I:=fibonacci_invariant (sz:=sz)).
   apply fold_left_accumulate_invariant_seq with (I:=fibonacci_invariant (sz:=sz)).
   { cbv [fibonacci_invariant]. ssplit; reflexivity. }
   { cbv [fibonacci_invariant].
