investigations/cava2/Types.v
@@ -27,7 +27,6 @@ Require Import Cava.Util.Vector.
 Inductive type :=
 | Unit : type
 | Bit  : type
-| Nat  : type
 | Vec  : type -> nat -> type
 | Pair : type -> type -> type
 .
@@ -40,76 +39,21 @@ Proof.
   apply Nat.eq_dec.
 Defined.
 
-Section RefinedLists.
-  Import ListNotations.
-
-  Notation rlist A n := {l : list A | Datatypes.length l = n}.
-
-  (* Do these exist somewhere *)
-  Lemma empty_list_with_Sn_length_is_false
-       : forall {t : Type} {n : nat} {x : list t},
-         Datatypes.length x = S n -> x = [] -> False.
-  Proof. intros; rewrite H0 in H; inversion H. Qed.
-
-  Lemma append_push_list_length
-       : forall {t : Type} {n : nat} {x0 : list t},
-         Datatypes.length x0 = S n ->
-         forall (x : t) (xs : list t), x0 = x :: xs -> Datatypes.length xs = n.
-  Proof. intros; rewrite H0 in H; cbn in *; congruence. Qed.
-
-  Definition hd_safe {t n} (ls: rlist t (S n)): (t * rlist t n) :=
-    let (ls', Hlen) := ls in
-    match ls' as ls'' return ls' = ls'' -> (t * rlist _ _) with
-    | [] => fun Heq => False_rect _ (empty_list_with_Sn_length_is_false Hlen Heq)
-    | x::xs => fun Heq => (x, exist _ xs (append_push_list_length Hlen x _ Heq))
-    end eq_refl.
-
-  Program Definition map {A B n} (f: A -> B) (ls: rlist A n): rlist B n :=
-    let (ls', Hlen) := ls in List.map f ls'.
-  Next Obligation.  rewrite map_length; reflexivity. Qed.
-
-  (* Lemma _ (tl ls : rlist A (n - 1)) _)) _ *)
-
-  Fixpoint ldrop {A} n (ls: list A): list A :=
-    match n with
-    | O => ls
-    | S n' => ldrop n' (tl ls)
-    end.
-
-  Program Fixpoint drop {A n} (m: nat) (ls: rlist A n) {struct m}: rlist A (n - m) :=
-    ldrop m ls.
-  Next Obligation.
-    revert m.
-
-    induction ls.
-    induction m.
-    - reflexivity.
-    - apply IHm.
-    - induction m; [reflexivity| apply IHls].
-  Qed.
-
-  Definition slice {A n} (start len: nat)
-      (ls: {l : list A | Datatypes.length l = n}):
-      if len <=? n - start then {l : list A | Datatypes.length l = len}
-      else unit :=
-    let (ls', Hlen) := ls in
-    if len <=? n - start then _ (drop start ls)
-    else tt.
-End.
-
-End RefinedLists.
-
 Fixpoint denote_type (t: type) :=
   match t with
   | Unit => unit
   | Bit => bool
-  | Nat => nat
-    (* Experience suggests to avoid vectors? What about refined lists - will the
-    * prop size grow and be an issue with proof? *)
-    (* One pro: Prop erasure in extraction means extracted terms are smaller
-     * than vecs *)
-  | Vec t n => {l: list (denote_type t) | List.length l = n}
+  | Vec t n => list (denote_type t)
   | Pair x y => (denote_type x * denote_type y)%type
+  end.
+
+Fixpoint eqb {t}: denote_type t -> denote_type t -> bool :=
+  match t return denote_type t -> denote_type t -> bool with
+  | Unit => fun _ _ => true
+  | Bit => fun x y => Bool.eqb x y
+  | Vec t n => fun x y =>
+    fold_right andb true (map (fun '(x,y) => eqb (t:=t) x y) (combine x y))
+  | Pair x y => fun '(x1,y1) '(x2,y2) => andb (eqb x1 x2) (eqb y1 y2)
   end.
 
 (* *)
@@ -117,11 +61,10 @@ Fixpoint denote1_type (t: type) :=
   match t with
   | Unit => unit
   | Bit => bool
-  | Nat => nat
   | Vec t n =>
     match t with
     | Bit => N
-    | _ => {l: list (denote1_type t) | List.length l = n}
+    | _ => list (denote1_type t)
     end
   | Pair x y => (denote1_type x * denote1_type y)%type
   end.
@@ -135,10 +78,25 @@ Fixpoint denote1_to_denote {t} : denote1_type t -> denote_type t :=
               -> denote1_type (Vec t1 n) -> denote_type (Vec t1 n))
     with
     | Bit => fun _ x =>
-      let v := N2Bv_sized n x in exist _ (Vector.to_list v) (to_list_length v)
+      let v := N2Bv_sized n x in Vector.to_list v
     | _ => fun f x => map f x
     end f
   | Pair x y => fun '(x,y) => (denote1_to_denote x, denote1_to_denote y)
+  | _ => id
+  end.
+
+Fixpoint denote_to_denote1 {t} : denote_type t -> denote1_type t :=
+  match t return denote_type t -> denote1_type t with
+  | Vec t n =>
+    let f := denote_to_denote1 in
+    match t as t1
+      return ((denote_type t1 -> denote1_type t1)
+              -> denote_type (Vec t1 n) -> denote1_type (Vec t1 n))
+    with
+    | Bit => fun _ x => Bv2N (Vector.of_list x)
+    | _ => fun f x => map f x
+    end f
+  | Pair x y => fun '(x,y) => (denote_to_denote1 x, denote_to_denote1 y)
   | _ => id
   end.
 
@@ -155,30 +113,49 @@ Fixpoint ntuple t n : type :=
   | S n => Pair t (ntuple t n)
   end.
 
-Definition vector_head {t n}: denote_type (Vec t (S n)) -> denote_type t * denote_type (Vec t n) := hd_safe.
-
-Fixpoint vector_as_tuple n t {struct n}: denote_type (Vec t (S n)) -> denote_type (ntuple t n) :=
-  match n with
-  | O => fun x => fst (vector_head x)
-  | S n' => fun ls =>
-    let '(hd,tl) := vector_head ls in
-    (hd, vector_as_tuple n' _ tl)
+Fixpoint default {t: type} : denote_type t :=
+  match t return denote_type t with
+  | Unit => tt
+  | Bit => false
+  | Vec t1 n => List.repeat default n
+  | Pair x y => (@default x, @default y)
   end.
-Definition vector_as_tuple1 n t (x: denote1_type (Vec t (S n))): denote_type (ntuple t n) :=
+
+Fixpoint default1 {t: type} : denote1_type t :=
+  match t return denote1_type t with
+  | Unit => tt
+  | Bit => false
+  | Vec t1 n =>
+    match t1 return denote1_type t1 -> denote1_type (Vec t1 n) with
+    | Bit => fun _ => 0%N
+    | _ => fun d => List.repeat d n
+    end default1
+  | Pair x y => (@default1 x, @default1 y)
+  end.
+
+Fixpoint vector_as_tuple n t {struct n}
+  : denote_type (Vec t (S n)) -> denote_type (ntuple t n) :=
+  match n with
+  | O => fun x => hd default x
+  | S n' => fun ls =>
+    (hd default ls, vector_as_tuple _ _ (tl ls))
+  end.
+
+Definition vector_as_tuple1 n t (x: denote1_type (Vec t (S n)))
+  : denote_type (ntuple t n) :=
   vector_as_tuple _ _ (denote1_to_denote x).
 
-Section test.
-  Import ListNotations.
-  Compute (vector_as_tuple1 _ _ (exist _ [0;1;2] _:denote1_type (Vec (BitVec 3) 3)))%N.
-  Compute (vector_as_tuple1 _ _ (exist _ [0;1;2] _:denote1_type (Vec (BitVec 3) 3)))%N.
-End test.
+(* Section test. *)
+(*   Import ListNotations. *)
+(*   Compute (vector_as_tuple1 _ _ ([0;1;2]:denote1_type (Vec (BitVec 3) 3)))%N. *)
+(* End test. *)
 
 Declare Scope circuit_type_scope.
 Delimit Scope circuit_type_scope with circuit_type.
 Open Scope circuit_type_scope.
-Notation "[ ]" := unit (format "[ ]") : circuit_type_scope.
-Notation "[ x ]" := (pair x unit) : circuit_type_scope.
-Notation "[ x ; y ; .. ; z ]" := (pair x (pair y .. (pair z unit) ..)) : circuit_type_scope.
-Notation "x ** y" := (pair x y)(at level 60, right associativity) : circuit_type_scope.
+Notation "[ ]" := Unit (format "[ ]") : circuit_type_scope.
+Notation "[ x ]" := (Pair x Unit) : circuit_type_scope.
+Notation "[ x ; y ; .. ; z ]" := (Pair x (Pair y .. (Pair z Unit) ..)) : circuit_type_scope.
+Notation "x ** y" := (Pair x y)(at level 60, right associativity) : circuit_type_scope.
 Notation "x ++ y" := (absorb_any x y) (at level 60, right associativity): circuit_type_scope.
 
